PCM in the ModSimPico

src/ModSimPico.v
@@ -4,13 +4,16 @@ Require Export Coq.Strings.String.
 Require Import Coq.Classes.RelationClasses.
 
 From Fairness Require Export ITreeLib FairBeh Mod.
-From Fairness Require Import pind5.
+From Fairness Require Import pind.
+From Fairness Require Import PCM.
 
 Set Implicit Arguments.
 
 
 
 Section PRIMIVIESIM.
+  Context `{M: URA.t}.
+
   Variable state_src: Type.
   Variable state_tgt: Type.
 
@@ -25,9 +28,6 @@ Section PRIMIVIESIM.
   Let srcE := ((@eventE _ident_src +' cE) +' sE state_src).
   Let tgtE := ((@eventE _ident_tgt +' cE) +' sE state_tgt).
 
-  Variable world: Type.
-  Variable world_le: world -> world -> Prop.
-
   Definition shared :=
     (TIdSet.t *
        TIdSet.t *
@@ -36,174 +36,175 @@ Section PRIMIVIESIM.
        state_src *
        state_tgt *
        wf_src.(T) *
-       world)%type.
+       URA.car)%type.
 
   Let shared_rel: Type := shared -> Prop.
 
   Variable I: shared_rel.
 
-  Variant __lsim R_src R_tgt (RR: R_src -> R_tgt -> shared_rel) (tid: thread_id)
-            (lsim: bool -> bool -> itree srcE R_src -> itree tgtE R_tgt -> shared_rel)
-            (_lsim: bool -> bool -> itree srcE R_src -> itree tgtE R_tgt -> shared_rel)
+  Variant __lsim R_src R_tgt (RR: R_src -> R_tgt -> URA.car -> URA.car -> shared_rel) (tid: thread_id)
+            (lsim: bool -> bool -> URA.car -> URA.car -> itree srcE R_src -> itree tgtE R_tgt -> shared_rel)
+            (_lsim: bool -> bool -> URA.car -> URA.car -> itree srcE R_src -> itree tgtE R_tgt -> shared_rel)
     :
-    bool -> bool -> itree srcE R_src -> itree tgtE R_tgt -> shared_rel :=
+    bool -> bool -> URA.car -> URA.car -> itree srcE R_src -> itree tgtE R_tgt -> shared_rel :=
   | lsim_ret
-      f_src f_tgt
-      ths tht im_src im_tgt st_src st_tgt o w
+      f_src f_tgt r_own r_ctx
+      ths tht im_src im_tgt st_src st_tgt o r_shared
       r_src r_tgt
-      (LSIM: RR r_src r_tgt (ths, tht, im_src, im_tgt, st_src, st_tgt, o, w))
+      (LSIM: RR r_src r_tgt r_own r_ctx (ths, tht, im_src, im_tgt, st_src, st_tgt, o, r_shared))
     :
-    __lsim RR tid lsim _lsim f_src f_tgt (Ret r_src) (Ret r_tgt) (ths, tht, im_src, im_tgt, st_src, st_tgt, o, w)
+    __lsim RR tid lsim _lsim f_src f_tgt r_own r_ctx (Ret r_src) (Ret r_tgt) (ths, tht, im_src, im_tgt, st_src, st_tgt, o, r_shared)
 
   | lsim_tauL
-      f_src f_tgt
-      ths tht im_src im_tgt st_src st_tgt o w
+      f_src f_tgt r_own r_ctx
+      ths tht im_src im_tgt st_src st_tgt o r_shared
       itr_src itr_tgt
-      (LSIM: _lsim true f_tgt itr_src itr_tgt (ths, tht, im_src, im_tgt, st_src, st_tgt, o, w))
+      (LSIM: _lsim true f_tgt r_own r_ctx itr_src itr_tgt (ths, tht, im_src, im_tgt, st_src, st_tgt, o, r_shared))
     :
-    __lsim RR tid lsim _lsim f_src f_tgt (Tau itr_src) itr_tgt (ths, tht, im_src, im_tgt, st_src, st_tgt, o, w)
+    __lsim RR tid lsim _lsim f_src f_tgt r_own r_ctx (Tau itr_src) itr_tgt (ths, tht, im_src, im_tgt, st_src, st_tgt, o, r_shared)
   | lsim_chooseL
-      f_src f_tgt
-      ths tht im_src im_tgt st_src st_tgt o w
+      f_src f_tgt r_own r_ctx
+      ths tht im_src im_tgt st_src st_tgt o r_shared
       X ktr_src itr_tgt
-      (LSIM: exists x, _lsim true f_tgt (ktr_src x) itr_tgt (ths, tht, im_src, im_tgt, st_src, st_tgt, o, w))
+      (LSIM: exists x, _lsim true f_tgt r_own r_ctx (ktr_src x) itr_tgt (ths, tht, im_src, im_tgt, st_src, st_tgt, o, r_shared))
     :
-    __lsim RR tid lsim _lsim f_src f_tgt (trigger (Choose X) >>= ktr_src) itr_tgt (ths, tht, im_src, im_tgt, st_src, st_tgt, o, w)
+    __lsim RR tid lsim _lsim f_src f_tgt r_own r_ctx (trigger (Choose X) >>= ktr_src) itr_tgt (ths, tht, im_src, im_tgt, st_src, st_tgt, o, r_shared)
   | lsim_putL
-      f_src f_tgt
-      ths tht im_src im_tgt st_src st_tgt o w
+      f_src f_tgt r_own r_ctx
+      ths tht im_src im_tgt st_src st_tgt o r_shared
       st ktr_src itr_tgt
-      (LSIM: _lsim true f_tgt (ktr_src tt) itr_tgt (ths, tht, im_src, im_tgt, st, st_tgt, o, w))
+      (LSIM: _lsim true f_tgt r_own r_ctx (ktr_src tt) itr_tgt (ths, tht, im_src, im_tgt, st, st_tgt, o, r_shared))
     :
-    __lsim RR tid lsim _lsim f_src f_tgt (trigger (Put st) >>= ktr_src) itr_tgt (ths, tht, im_src, im_tgt, st_src, st_tgt, o, w)
+    __lsim RR tid lsim _lsim f_src f_tgt r_own r_ctx (trigger (Put st) >>= ktr_src) itr_tgt (ths, tht, im_src, im_tgt, st_src, st_tgt, o, r_shared)
   | lsim_getL
-      f_src f_tgt
-      ths tht im_src im_tgt st_src st_tgt o w
+      f_src f_tgt r_own r_ctx
+      ths tht im_src im_tgt st_src st_tgt o r_shared
       ktr_src itr_tgt
-      (LSIM: _lsim true f_tgt (ktr_src st_src) itr_tgt (ths, tht, im_src, im_tgt, st_src, st_tgt, o, w))
+      (LSIM: _lsim true f_tgt r_own r_ctx (ktr_src st_src) itr_tgt (ths, tht, im_src, im_tgt, st_src, st_tgt, o, r_shared))
     :
-    __lsim RR tid lsim _lsim f_src f_tgt (trigger (@Get _) >>= ktr_src) itr_tgt (ths, tht, im_src, im_tgt, st_src, st_tgt, o, w)
+    __lsim RR tid lsim _lsim f_src f_tgt r_own r_ctx (trigger (@Get _) >>= ktr_src) itr_tgt (ths, tht, im_src, im_tgt, st_src, st_tgt, o, r_shared)
   | lsim_tidL
-      f_src f_tgt
-      ths tht im_src im_tgt st_src st_tgt o w
+      f_src f_tgt r_own r_ctx
+      ths tht im_src im_tgt st_src st_tgt o r_shared
       ktr_src itr_tgt
-      (LSIM: _lsim true f_tgt (ktr_src tid) itr_tgt (ths, tht, im_src, im_tgt, st_src, st_tgt, o, w))
+      (LSIM: _lsim true f_tgt r_own r_ctx (ktr_src tid) itr_tgt (ths, tht, im_src, im_tgt, st_src, st_tgt, o, r_shared))
     :
-    __lsim RR tid lsim _lsim f_src f_tgt (trigger (GetTid) >>= ktr_src) itr_tgt (ths, tht, im_src, im_tgt, st_src, st_tgt, o, w)
+    __lsim RR tid lsim _lsim f_src f_tgt r_own r_ctx (trigger (GetTid) >>= ktr_src) itr_tgt (ths, tht, im_src, im_tgt, st_src, st_tgt, o, r_shared)
   | lsim_UB
-      f_src f_tgt
-      ths tht im_src im_tgt st_src st_tgt o w
+      f_src f_tgt r_own r_ctx
+      ths tht im_src im_tgt st_src st_tgt o r_shared
       ktr_src itr_tgt
     :
-    __lsim RR tid lsim _lsim f_src f_tgt (trigger (Undefined) >>= ktr_src) itr_tgt (ths, tht, im_src, im_tgt, st_src, st_tgt, o, w)
+    __lsim RR tid lsim _lsim f_src f_tgt r_own r_ctx (trigger (Undefined) >>= ktr_src) itr_tgt (ths, tht, im_src, im_tgt, st_src, st_tgt, o, r_shared)
   | lsim_fairL
-      f_src f_tgt
-      ths tht im_src0 im_tgt st_src st_tgt o w
+      f_src f_tgt r_own r_ctx
+      ths tht im_src0 im_tgt st_src st_tgt o r_shared
       f ktr_src itr_tgt
       (LSIM: exists im_src1,
           (<<FAIR: fair_update im_src0 im_src1 (sum_fmap_r f)>>) /\
-            (<<LSIM: _lsim true f_tgt (ktr_src tt) itr_tgt (ths, tht, im_src1, im_tgt, st_src, st_tgt, o, w)>>))
+            (<<LSIM: _lsim true f_tgt r_own r_ctx (ktr_src tt) itr_tgt (ths, tht, im_src1, im_tgt, st_src, st_tgt, o, r_shared)>>))
     :
-    __lsim RR tid lsim _lsim f_src f_tgt (trigger (Fair f) >>= ktr_src) itr_tgt (ths, tht, im_src0, im_tgt, st_src, st_tgt, o, w)
+    __lsim RR tid lsim _lsim f_src f_tgt r_own r_ctx (trigger (Fair f) >>= ktr_src) itr_tgt (ths, tht, im_src0, im_tgt, st_src, st_tgt, o, r_shared)
 
   | lsim_tauR
-      f_src f_tgt
-      ths tht im_src im_tgt st_src st_tgt o w
+      f_src f_tgt r_own r_ctx
+      ths tht im_src im_tgt st_src st_tgt o r_shared
       itr_src itr_tgt
-      (LSIM: _lsim f_src true itr_src itr_tgt (ths, tht, im_src, im_tgt, st_src, st_tgt, o, w))
+      (LSIM: _lsim f_src true r_own r_ctx itr_src itr_tgt (ths, tht, im_src, im_tgt, st_src, st_tgt, o, r_shared))
     :
-    __lsim RR tid lsim _lsim f_src f_tgt itr_src (Tau itr_tgt) (ths, tht, im_src, im_tgt, st_src, st_tgt, o, w)
+    __lsim RR tid lsim _lsim f_src f_tgt r_own r_ctx itr_src (Tau itr_tgt) (ths, tht, im_src, im_tgt, st_src, st_tgt, o, r_shared)
   | lsim_chooseR
-      f_src f_tgt
-      ths tht im_src im_tgt st_src st_tgt o w
+      f_src f_tgt r_own r_ctx
+      ths tht im_src im_tgt st_src st_tgt o r_shared
       X itr_src ktr_tgt
-      (LSIM: forall x, _lsim f_src true itr_src (ktr_tgt x) (ths, tht, im_src, im_tgt, st_src, st_tgt, o, w))
+      (LSIM: forall x, _lsim f_src true r_own r_ctx itr_src (ktr_tgt x) (ths, tht, im_src, im_tgt, st_src, st_tgt, o, r_shared))
     :
-    __lsim RR tid lsim _lsim f_src f_tgt itr_src (trigger (Choose X) >>= ktr_tgt) (ths, tht, im_src, im_tgt, st_src, st_tgt, o, w)
+    __lsim RR tid lsim _lsim f_src f_tgt r_own r_ctx itr_src (trigger (Choose X) >>= ktr_tgt) (ths, tht, im_src, im_tgt, st_src, st_tgt, o, r_shared)
   | lsim_putR
-      f_src f_tgt
-      ths tht im_src im_tgt st_src st_tgt o w
+      f_src f_tgt r_own r_ctx
+      ths tht im_src im_tgt st_src st_tgt o r_shared
       st itr_src ktr_tgt
-      (LSIM: _lsim f_src true itr_src (ktr_tgt tt) (ths, tht, im_src, im_tgt, st_src, st, o, w))
+      (LSIM: _lsim f_src true r_own r_ctx itr_src (ktr_tgt tt) (ths, tht, im_src, im_tgt, st_src, st, o, r_shared))
     :
-    __lsim RR tid lsim _lsim f_src f_tgt itr_src (trigger (Put st) >>= ktr_tgt) (ths, tht, im_src, im_tgt, st_src, st_tgt, o, w)
+    __lsim RR tid lsim _lsim f_src f_tgt r_own r_ctx itr_src (trigger (Put st) >>= ktr_tgt) (ths, tht, im_src, im_tgt, st_src, st_tgt, o, r_shared)
   | lsim_getR
-      f_src f_tgt
-      ths tht im_src im_tgt st_src st_tgt o w
+      f_src f_tgt r_own r_ctx
+      ths tht im_src im_tgt st_src st_tgt o r_shared
       itr_src ktr_tgt
-      (LSIM: _lsim f_src true itr_src (ktr_tgt st_tgt) (ths, tht, im_src, im_tgt, st_src, st_tgt, o, w))
+      (LSIM: _lsim f_src true r_own r_ctx itr_src (ktr_tgt st_tgt) (ths, tht, im_src, im_tgt, st_src, st_tgt, o, r_shared))
     :
-    __lsim RR tid lsim _lsim f_src f_tgt itr_src (trigger (@Get _) >>= ktr_tgt) (ths, tht, im_src, im_tgt, st_src, st_tgt, o, w)
+    __lsim RR tid lsim _lsim f_src f_tgt r_own r_ctx itr_src (trigger (@Get _) >>= ktr_tgt) (ths, tht, im_src, im_tgt, st_src, st_tgt, o, r_shared)
   | lsim_tidR
-      f_src f_tgt
-      ths tht im_src im_tgt st_src st_tgt o w
+      f_src f_tgt r_own r_ctx
+      ths tht im_src im_tgt st_src st_tgt o r_shared
       itr_src ktr_tgt
-      (LSIM: _lsim f_src true itr_src (ktr_tgt tid) (ths, tht, im_src, im_tgt, st_src, st_tgt, o, w))
+      (LSIM: _lsim f_src true r_own r_ctx itr_src (ktr_tgt tid) (ths, tht, im_src, im_tgt, st_src, st_tgt, o, r_shared))
     :
-    __lsim RR tid lsim _lsim f_src f_tgt itr_src (trigger (GetTid) >>= ktr_tgt) (ths, tht, im_src, im_tgt, st_src, st_tgt, o, w)
+    __lsim RR tid lsim _lsim f_src f_tgt r_own r_ctx itr_src (trigger (GetTid) >>= ktr_tgt) (ths, tht, im_src, im_tgt, st_src, st_tgt, o, r_shared)
   | lsim_fairR
-      f_src f_tgt
-      ths tht im_src im_tgt0 st_src st_tgt o w
+      f_src f_tgt r_own r_ctx
+      ths tht im_src im_tgt0 st_src st_tgt o r_shared
       f itr_src ktr_tgt
       (LSIM: forall im_tgt1
                    (FAIR: fair_update im_tgt0 im_tgt1 (sum_fmap_r f)),
-          (<<LSIM: _lsim f_src true itr_src (ktr_tgt tt) (ths, tht, im_src, im_tgt1, st_src, st_tgt, o, w)>>))
+          (<<LSIM: _lsim f_src true r_own r_ctx itr_src (ktr_tgt tt) (ths, tht, im_src, im_tgt1, st_src, st_tgt, o, r_shared)>>))
     :
-    __lsim RR tid lsim _lsim f_src f_tgt itr_src (trigger (Fair f) >>= ktr_tgt) (ths, tht, im_src, im_tgt0, st_src, st_tgt, o, w)
+    __lsim RR tid lsim _lsim f_src f_tgt r_own r_ctx itr_src (trigger (Fair f) >>= ktr_tgt) (ths, tht, im_src, im_tgt0, st_src, st_tgt, o, r_shared)
 
   | lsim_observe
-      f_src f_tgt
-      ths tht im_src im_tgt st_src st_tgt o w
+      f_src f_tgt r_own r_ctx
+      ths tht im_src im_tgt st_src st_tgt o r_shared
       fn args ktr_src ktr_tgt
       (LSIM: forall ret,
-          lsim true true (ktr_src ret) (ktr_tgt ret) (ths, tht, im_src, im_tgt, st_src, st_tgt, o, w))
+          lsim true true r_own r_ctx (ktr_src ret) (ktr_tgt ret) (ths, tht, im_src, im_tgt, st_src, st_tgt, o, r_shared))
     :
-    __lsim RR tid lsim _lsim f_src f_tgt (trigger (Observe fn args) >>= ktr_src) (trigger (Observe fn args) >>= ktr_tgt) (ths, tht, im_src, im_tgt, st_src, st_tgt, o, w)
+    __lsim RR tid lsim _lsim f_src f_tgt r_own r_ctx (trigger (Observe fn args) >>= ktr_src) (trigger (Observe fn args) >>= ktr_tgt) (ths, tht, im_src, im_tgt, st_src, st_tgt, o, r_shared)
 
   | lsim_sync
-      f_src f_tgt
-      ths0 tht0 im_src0 im_tgt0 st_src0 st_tgt0 o w
-      o0 w0 ktr_src ktr_tgt
-      (INV: I (ths0, tht0, im_src0, im_tgt0, st_src0, st_tgt0, o0, w0))
-      (WORLD: world_le w w0)
+      f_src f_tgt r_own0 r_ctx0
+      ths0 tht0 im_src0 im_tgt0 st_src0 st_tgt0 o r_shared0
+      o0 r_own1 ktr_src ktr_tgt
+      (INV: I (ths0, tht0, im_src0, im_tgt0, st_src0, st_tgt0, o0, r_shared0))
+      (VALID: URA.wf (r_shared0 ⋅ r_own0 ⋅ r_ctx0))
       (STUTTER: wf_src.(lt) o0 o)
-      (LSIM: forall ths1 tht1 im_src1 im_tgt1 st_src1 st_tgt1 o1 w1
-                   (INV: I (ths1, tht1, im_src1, im_tgt1, st_src1, st_tgt1, o1, w1))
-                   (WORLD: world_le w0 w1)
-                   im_tgt2
-                   (TGT: fair_update im_tgt1 im_tgt2 (sum_fmap_l (tids_fmap tid tht1))),
-          lsim true true (trigger (Yield) >>= ktr_src) (ktr_tgt tt) (ths1, tht1, im_src1, im_tgt2, st_src1, st_tgt1, o1, w1))
+      (LSIM: forall ths1 tht1 im_src1 im_tgt1 st_src1 st_tgt1 o1 r_shared1 r_ctx1
+                    (INV: I (ths1, tht1, im_src1, im_tgt1, st_src1, st_tgt1, o1, r_shared1))
+                    (VALID: URA.wf (r_shared1 ⋅ r_own0 ⋅ r_ctx1))
+                    im_tgt2
+                    (TGT: fair_update im_tgt1 im_tgt2 (sum_fmap_l (tids_fmap tid tht1))),
+          lsim true true r_own1 r_ctx1 (trigger (Yield) >>= ktr_src) (ktr_tgt tt) (ths1, tht1, im_src1, im_tgt2, st_src1, st_tgt1, o1, r_shared1))
     :
-    __lsim RR tid lsim _lsim f_src f_tgt (trigger (Yield) >>= ktr_src) (trigger (Yield) >>= ktr_tgt) (ths0, tht0, im_src0, im_tgt0, st_src0, st_tgt0, o, w)
+    __lsim RR tid lsim _lsim f_src f_tgt r_own0 r_ctx0 (trigger (Yield) >>= ktr_src) (trigger (Yield) >>= ktr_tgt) (ths0, tht0, im_src0, im_tgt0, st_src0, st_tgt0, o, r_shared0)
   | lsim_yieldL
-      f_src f_tgt
+      f_src f_tgt r_own r_ctx
       ths tht im_src0 im_tgt st_src st_tgt o0 w
       ktr_src itr_tgt
       (LSIM: exists im_src1 o1,
           (<<FAIR: fair_update im_src0 im_src1 (sum_fmap_l (tids_fmap tid ths))>>) /\
-            (<<LSIM: _lsim true f_tgt (ktr_src tt) itr_tgt (ths, tht, im_src1, im_tgt, st_src, st_tgt, o1, w)>>))
+            (<<LSIM: _lsim true f_tgt r_own r_ctx (ktr_src tt) itr_tgt (ths, tht, im_src1, im_tgt, st_src, st_tgt, o1, w)>>))
     :
-    __lsim RR tid lsim _lsim f_src f_tgt (trigger (Yield) >>= ktr_src) itr_tgt (ths, tht, im_src0, im_tgt, st_src, st_tgt, o0, w)
+    __lsim RR tid lsim _lsim f_src f_tgt r_own r_ctx (trigger (Yield) >>= ktr_src) itr_tgt (ths, tht, im_src0, im_tgt, st_src, st_tgt, o0, w)
 
   | lsim_progress
-      ths tht im_src im_tgt st_src st_tgt o w
+      r_own r_ctx
+      ths tht im_src im_tgt st_src st_tgt o r_shared
       itr_src itr_tgt
-      (LSIM: lsim false false itr_src itr_tgt (ths, tht, im_src, im_tgt, st_src, st_tgt, o, w))
+      (LSIM: lsim false false r_own r_ctx itr_src itr_tgt (ths, tht, im_src, im_tgt, st_src, st_tgt, o, r_shared))
     :
-    __lsim RR tid lsim _lsim true true itr_src itr_tgt (ths, tht, im_src, im_tgt, st_src, st_tgt, o, w)
+    __lsim RR tid lsim _lsim true true r_own r_ctx itr_src itr_tgt (ths, tht, im_src, im_tgt, st_src, st_tgt, o, r_shared)
   .
 
-  Definition lsim R_src R_tgt (RR: R_src -> R_tgt -> shared_rel) (tid: thread_id):
-    bool -> bool -> itree srcE R_src -> itree tgtE R_tgt -> shared_rel :=
-    paco5 (fun r => pind5 (__lsim RR tid r) top5) bot5.
+  Definition lsim R_src R_tgt (RR: R_src -> R_tgt -> URA.car -> URA.car -> shared_rel) (tid: thread_id):
+    bool -> bool -> URA.car -> URA.car -> itree srcE R_src -> itree tgtE R_tgt -> shared_rel :=
+    paco7 (fun r => pind7 (__lsim RR tid r) top7) bot7.
 
-  Lemma __lsim_mon R0 R1 (RR: R0 -> R1 -> shared_rel) tid:
-    forall r r' (LE: r <5= r'), (__lsim RR tid r) <6= (__lsim RR tid r').
+  Lemma __lsim_mon R0 R1 (RR: R0 -> R1 -> URA.car -> URA.car -> shared_rel) tid:
+    forall r r' (LE: r <7= r'), (__lsim RR tid r) <8= (__lsim RR tid r').
   Proof.
     ii. inv PR; econs; eauto.
   Qed.
 
-  Lemma _lsim_mon R0 R1 (RR: R0 -> R1 -> shared_rel) tid: forall r, monotone5 (__lsim RR tid r).
+  Lemma _lsim_mon R0 R1 (RR: R0 -> R1 -> URA.car -> URA.car -> shared_rel) tid: forall r, monotone7 (__lsim RR tid r).
   Proof.
     ii. inv IN; econs; eauto.
     { des. eauto. }
@@ -212,253 +213,254 @@ Section PRIMIVIESIM.
     { des. esplits; eauto. }
   Qed.
 
-  Lemma lsim_mon R0 R1 (RR: R0 -> R1 -> shared_rel) tid: forall q, monotone5 (fun r => pind5 (__lsim RR tid r) q).
+  Lemma lsim_mon R0 R1 (RR: R0 -> R1 -> URA.car -> URA.car -> shared_rel) tid: forall q, monotone7 (fun r => pind7 (__lsim RR tid r) q).
   Proof.
-    ii. eapply pind5_mon_gen; eauto.
+    ii. eapply pind7_mon_gen; eauto.
     ii. eapply __lsim_mon; eauto.
   Qed.
 
 
   Lemma lsim_reset_prog
-        R0 R1 (RR: R0 -> R1 -> shared_rel) tid
+        R0 R1 (RR: R0 -> R1 -> URA.car -> URA.car-> shared_rel) tid
         src tgt shr
         ps0 pt0 ps1 pt1
-        (LSIM: lsim RR tid ps1 pt1 src tgt shr)
+        r_own r_ctx
+        (LSIM: lsim RR tid ps1 pt1 r_own r_ctx src tgt shr)
         (SRC: ps1 = true -> ps0 = true)
         (TGT: pt1 = true -> pt0 = true)
     :
-    lsim RR tid ps0 pt0 src tgt shr.
+    lsim RR tid ps0 pt0 r_own r_ctx src tgt shr.
   Proof.
     revert_until tid. pcofix CIH. i.
     move LSIM before CIH. revert_until LSIM. punfold LSIM.
     2:{ eapply lsim_mon. }
-    eapply pind5_acc in LSIM.
+    eapply pind7_acc in LSIM.
 
-    { instantiate (1:= (fun ps1 pt1 src tgt shr =>
+    { instantiate (1:= (fun ps1 pt1 r_own r_ctx src tgt shr =>
                           forall ps0 pt0 : bool,
                             (ps1 = true -> ps0 = true) ->
                             (pt1 = true -> pt0 = true) ->
-                            paco5
+                            paco7
                               (fun
-                                  r0 : rel5 bool (fun _ : bool => bool) (fun _ _ : bool => itree srcE R0)
-                                            (fun (_ _ : bool) (_ : itree srcE R0) => itree tgtE R1)
-                                            (fun (_ _ : bool) (_ : itree srcE R0) (_ : itree tgtE R1) => shared) =>
-                                  pind5 (__lsim RR tid r0) top5) r ps0 pt0 src tgt shr)) in LSIM; auto. }
+                                  r0 =>
+                                  pind7 (__lsim RR tid r0) top7) r ps0 pt0 r_own r_ctx src tgt shr)) in LSIM; auto. }
 
-    ss. clear ps1 pt1 src tgt shr LSIM.
-    intros rr DEC IH ps1 pt1 src tgt shr LSIM. clear DEC.
+    ss. clear ps1 pt1 r_own r_ctx src tgt shr LSIM.
+    intros rr DEC IH ps1 pt1 r_own r_ctx src tgt shr LSIM. clear DEC.
     intros ps0 pt0 SRC TGT.
-    eapply pind5_unfold in LSIM.
+    eapply pind7_unfold in LSIM.
     2:{ eapply _lsim_mon. }
     inv LSIM.
 
-    { pfold. eapply pind5_fold. econs; eauto. }
+    { pfold. eapply pind7_fold. econs; eauto. }
 
     { destruct LSIM0 as [LSIM0 IND]. clear LSIM0.
-      pfold. eapply pind5_fold. eapply lsim_tauL. split; ss.
+      pfold. eapply pind7_fold. eapply lsim_tauL. split; ss.
       hexploit IH. eauto. all: eauto. i. punfold H. eapply lsim_mon.
     }
 
-    { des. pfold. eapply pind5_fold. eapply lsim_chooseL. esplits; eauto. split; ss.
+    { des. pfold. eapply pind7_fold. eapply lsim_chooseL. esplits; eauto. split; ss.
       destruct LSIM0 as [LSIM0 IND]. hexploit IH; eauto. i. punfold H. eapply lsim_mon.
     }
 
-    { pfold. eapply pind5_fold. eapply lsim_putL. split; ss.
+    { pfold. eapply pind7_fold. eapply lsim_putL. split; ss.
       destruct LSIM0 as [LSIM0 IND]. hexploit IH; eauto. i. punfold H. eapply lsim_mon.
     }
 
-    { pfold. eapply pind5_fold. eapply lsim_getL. split; ss.
+    { pfold. eapply pind7_fold. eapply lsim_getL. split; ss.
       destruct LSIM0 as [LSIM0 IND]. hexploit IH; eauto. i. punfold H. eapply lsim_mon.
     }
 
-    { pfold. eapply pind5_fold. eapply lsim_tidL. split; ss.
+    { pfold. eapply pind7_fold. eapply lsim_tidL. split; ss.
       destruct LSIM0 as [LSIM0 IND]. hexploit IH; eauto. i. punfold H. eapply lsim_mon.
     }
 
-    { pfold. eapply pind5_fold. eapply lsim_UB. }
+    { pfold. eapply pind7_fold. eapply lsim_UB. }
 
-    { des. pfold. eapply pind5_fold. eapply lsim_fairL. esplits; eauto. split; ss.
+    { des. pfold. eapply pind7_fold. eapply lsim_fairL. esplits; eauto. split; ss.
       destruct LSIM as [LSIM IND]. hexploit IH; eauto. i. punfold H. eapply lsim_mon.
     }
 
     { destruct LSIM0 as [LSIM0 IND]. clear LSIM0.
-      pfold. eapply pind5_fold. eapply lsim_tauR. split; ss.
+      pfold. eapply pind7_fold. eapply lsim_tauR. split; ss.
       hexploit IH. eauto. all: eauto. i. punfold H. eapply lsim_mon.
     }
 
-    { pfold. eapply pind5_fold. eapply lsim_chooseR. i. split; ss. specialize (LSIM0 x).
+    { pfold. eapply pind7_fold. eapply lsim_chooseR. i. split; ss. specialize (LSIM0 x).
       destruct LSIM0 as [LSIM0 IND]. hexploit IH; eauto. i. punfold H. eapply lsim_mon.
     }
 
-    { pfold. eapply pind5_fold. eapply lsim_putR. split; ss.
+    { pfold. eapply pind7_fold. eapply lsim_putR. split; ss.
       destruct LSIM0 as [LSIM0 IND]. hexploit IH; eauto. i. punfold H. eapply lsim_mon.
     }
 
-    { pfold. eapply pind5_fold. eapply lsim_getR. split; ss.
+    { pfold. eapply pind7_fold. eapply lsim_getR. split; ss.
       destruct LSIM0 as [LSIM0 IND]. hexploit IH; eauto. i. punfold H. eapply lsim_mon.
     }
 
-    { pfold. eapply pind5_fold. eapply lsim_tidR. split; ss.
+    { pfold. eapply pind7_fold. eapply lsim_tidR. split; ss.
       destruct LSIM0 as [LSIM0 IND]. hexploit IH; eauto. i. punfold H. eapply lsim_mon.
     }
 
-    { pfold. eapply pind5_fold. eapply lsim_fairR. i. split; ss. specialize (LSIM0 _ FAIR).
+    { pfold. eapply pind7_fold. eapply lsim_fairR. i. split; ss. specialize (LSIM0 _ FAIR).
       des. destruct LSIM0 as [LSIM0 IND]. hexploit IH; eauto. i. punfold H. eapply lsim_mon.
     }
 
-    { pfold. eapply pind5_fold. eapply lsim_observe. i. eapply upaco5_mon_bot; eauto. }
+    { pfold. eapply pind7_fold. eapply lsim_observe. i. eapply upaco7_mon_bot; eauto. }
 
-    { pfold. eapply pind5_fold. eapply lsim_sync; eauto. i. eapply upaco5_mon_bot; eauto. }
+    { pfold. eapply pind7_fold. eapply lsim_sync; eauto. i. eapply upaco7_mon_bot; eauto. }
 
-    { des. pfold. eapply pind5_fold. eapply lsim_yieldL. esplits; eauto. split; ss.
+    { des. pfold. eapply pind7_fold. eapply lsim_yieldL. esplits; eauto. split; ss.
       destruct LSIM as [LSIM IND]. hexploit IH; eauto. i. punfold H. eapply lsim_mon.
     }
 
     { pclearbot. hexploit SRC; ss; i. hexploit TGT; ss; i. clarify.
-      pfold. eapply pind5_fold. eapply lsim_progress. right. eapply CIH. eauto. all: ss. }
+      pfold. eapply pind7_fold. eapply lsim_progress. right. eapply CIH. eauto. all: ss. }
 
   Qed.
 
   Lemma lsim_set_prog
-        R0 R1 (RR: R0 -> R1 -> shared_rel) tid
+        R0 R1 (RR: R0 -> R1 -> URA.car -> URA.car -> shared_rel) tid
         src tgt shr
-        (LSIM: lsim RR tid true true src tgt shr)
+        r_own r_ctx
+        (LSIM: lsim RR tid true true r_own r_ctx src tgt shr)
     :
-    forall ps pt, lsim RR tid ps pt src tgt shr.
+    forall ps pt, lsim RR tid ps pt r_own r_ctx src tgt shr.
   Proof.
     i. revert_until tid. pcofix CIH. i.
     remember true as ps0 in LSIM at 1. remember true as pt0 in LSIM at 1.
     move LSIM before CIH. revert_until LSIM. punfold LSIM.
     2:{ eapply lsim_mon. }
-    eapply pind5_acc in LSIM.
+    eapply pind7_acc in LSIM.
 
-    { instantiate (1:= (fun ps0 pt0 src tgt shr =>
+    { instantiate (1:= (fun ps0 pt0 r_own r_ctx src tgt shr =>
                           ps0 = true ->
                           pt0 = true ->
                           forall ps pt : bool,
-                            paco5
+                            paco7
                               (fun
-                                  r0 : rel5 bool (fun _ : bool => bool) (fun _ _ : bool => itree srcE R0)
-                                            (fun (_ _ : bool) (_ : itree srcE R0) => itree tgtE R1)
-                                            (fun (_ _ : bool) (_ : itree srcE R0) (_ : itree tgtE R1) => shared) =>
-                                  pind5 (__lsim RR tid r0) top5) r ps pt src tgt shr)) in LSIM; auto. }
+                                  r0 =>
+                                  pind7 (__lsim RR tid r0) top7) r ps pt r_own r_ctx src tgt shr)) in LSIM; auto. }
 
-    ss. clear ps0 pt0 src tgt shr LSIM.
-    intros rr DEC IH gps gpt src tgt shr LSIM. clear DEC.
+    ss. clear ps0 pt0 r_own r_ctx src tgt shr LSIM.
+    intros rr DEC IH gps gpt r_own r_ctx src tgt shr LSIM. clear DEC.
     intros Egps Egpt ps pt.
-    eapply pind5_unfold in LSIM.
+    eapply pind7_unfold in LSIM.
     2:{ eapply _lsim_mon. }
     inv LSIM.
 
-    { pfold. eapply pind5_fold. econs; eauto. }
+    { pfold. eapply pind7_fold. econs; eauto. }
 
     { destruct LSIM0 as [LSIM0 IND]. clear LSIM0.
-      pfold. eapply pind5_fold. eapply lsim_tauL. split; ss.
+      pfold. eapply pind7_fold. eapply lsim_tauL. split; ss.
       hexploit IH. eauto. all: eauto. i. punfold H. eapply lsim_mon.
     }
 
-    { des. pfold. eapply pind5_fold. eapply lsim_chooseL. esplits; eauto. split; ss.
+    { des. pfold. eapply pind7_fold. eapply lsim_chooseL. esplits; eauto. split; ss.
       destruct LSIM0 as [LSIM0 IND]. hexploit IH; eauto. i. punfold H. eapply lsim_mon.
     }
 
-    { pfold. eapply pind5_fold. eapply lsim_putL. split; ss.
+    { pfold. eapply pind7_fold. eapply lsim_putL. split; ss.
       destruct LSIM0 as [LSIM0 IND]. hexploit IH; eauto. i. punfold H. eapply lsim_mon.
     }
 
-    { pfold. eapply pind5_fold. eapply lsim_getL. split; ss.
+    { pfold. eapply pind7_fold. eapply lsim_getL. split; ss.
       destruct LSIM0 as [LSIM0 IND]. hexploit IH; eauto. i. punfold H. eapply lsim_mon.
     }
 
-    { pfold. eapply pind5_fold. eapply lsim_tidL. split; ss.
+    { pfold. eapply pind7_fold. eapply lsim_tidL. split; ss.
       destruct LSIM0 as [LSIM0 IND]. hexploit IH; eauto. i. punfold H. eapply lsim_mon.
     }
 
-    { pfold. eapply pind5_fold. eapply lsim_UB. }
+    { pfold. eapply pind7_fold. eapply lsim_UB. }
 
-    { des. pfold. eapply pind5_fold. eapply lsim_fairL. esplits; eauto. split; ss.
+    { des. pfold. eapply pind7_fold. eapply lsim_fairL. esplits; eauto. split; ss.
       destruct LSIM as [LSIM IND]. hexploit IH; eauto. i. punfold H. eapply lsim_mon.
     }
 
     { destruct LSIM0 as [LSIM0 IND]. clear LSIM0.
-      pfold. eapply pind5_fold. eapply lsim_tauR. split; ss.
+      pfold. eapply pind7_fold. eapply lsim_tauR. split; ss.
       hexploit IH. eauto. all: eauto. i. punfold H. eapply lsim_mon.
     }
 
-    { pfold. eapply pind5_fold. eapply lsim_chooseR. i. split; ss. specialize (LSIM0 x).
+    { pfold. eapply pind7_fold. eapply lsim_chooseR. i. split; ss. specialize (LSIM0 x).
       destruct LSIM0 as [LSIM0 IND]. hexploit IH; eauto. i. punfold H. eapply lsim_mon.
     }
 
-    { pfold. eapply pind5_fold. eapply lsim_putR. split; ss.
+    { pfold. eapply pind7_fold. eapply lsim_putR. split; ss.
       destruct LSIM0 as [LSIM0 IND]. hexploit IH; eauto. i. punfold H. eapply lsim_mon.
     }
 
-    { pfold. eapply pind5_fold. eapply lsim_getR. split; ss.
+    { pfold. eapply pind7_fold. eapply lsim_getR. split; ss.
       destruct LSIM0 as [LSIM0 IND]. hexploit IH; eauto. i. punfold H. eapply lsim_mon.
     }
 
-    { pfold. eapply pind5_fold. eapply lsim_tidR. split; ss.
+    { pfold. eapply pind7_fold. eapply lsim_tidR. split; ss.
       destruct LSIM0 as [LSIM0 IND]. hexploit IH; eauto. i. punfold H. eapply lsim_mon.
     }
 
-    { pfold. eapply pind5_fold. eapply lsim_fairR. i. split; ss. specialize (LSIM0 _ FAIR).
+    { pfold. eapply pind7_fold. eapply lsim_fairR. i. split; ss. specialize (LSIM0 _ FAIR).
       des. destruct LSIM0 as [LSIM0 IND]. hexploit IH; eauto. i. punfold H. eapply lsim_mon.
     }
 
-    { pfold. eapply pind5_fold. eapply lsim_observe. i. eapply upaco5_mon_bot; eauto. }
+    { pfold. eapply pind7_fold. eapply lsim_observe. i. eapply upaco7_mon_bot; eauto. }
 
-    { pfold. eapply pind5_fold. eapply lsim_sync; eauto. i. eapply upaco5_mon_bot; eauto. }
+    { pfold. eapply pind7_fold. eapply lsim_sync; eauto. i. eapply upaco7_mon_bot; eauto. }
 
-    { des. pfold. eapply pind5_fold. eapply lsim_yieldL. esplits; eauto. split; ss.
+    { des. pfold. eapply pind7_fold. eapply lsim_yieldL. esplits; eauto. split; ss.
       destruct LSIM as [LSIM IND]. hexploit IH; eauto. i. punfold H. eapply lsim_mon.
     }
 
-    { pclearbot. eapply paco5_mon_bot. eapply lsim_reset_prog. eauto. all: ss. }
+    { pclearbot. eapply paco7_mon_bot. eapply lsim_reset_prog. eauto. all: ss. }
 
   Qed.
 
-  Definition local_RR {R0 R1} (RR: R0 -> R1 -> Prop) tid :=
-    fun (r_src: R0) (r_tgt: R1) '(ths2, tht2, im_src1, im_tgt1, st_src1, st_tgt1, o1, w1) =>
-      (exists ths3 tht3 o2 w2,
+  Definition local_RR {R0 R1} (RR: R0 -> R1 -> Prop) tid:
+    R0 -> R1 -> URA.car -> URA.car -> shared_rel :=
+    fun (r_src: R0) (r_tgt: R1) (r_own1: URA.car) (r_ctx: URA.car) '(ths2, tht2, im_src1, im_tgt1, st_src1, st_tgt1, o1, r_shared1) =>
+      (exists ths3 tht3 o2 r_own2 r_shared2,
           (<<THSR: NatMap.remove tid ths2 = ths3>>) /\
             (<<THTR: NatMap.remove tid tht2 = tht3>>) /\
-            (<<WORLD: world_le w1 w2>>) /\
+            (<<VALID: URA.wf (r_shared2 ⋅ r_own2 ⋅ r_ctx)>>) /\
             (<<STUTTER: wf_src.(lt) o2 o1>>) /\
-            (<<INV: I (ths3, tht3, im_src1, im_tgt1, st_src1, st_tgt1, o2, w2)>>) /\
+            (<<INV: I (ths3, tht3, im_src1, im_tgt1, st_src1, st_tgt1, o2, r_shared2)>>) /\
             (<<RET: RR r_src r_tgt>>)).
 
   Definition local_sim {R0 R1} (RR: R0 -> R1 -> Prop) src tgt :=
-    forall ths0 tht0 im_src0 im_tgt0 st_src0 st_tgt0 o0 w0
-      (INV: I (ths0, tht0, im_src0, im_tgt0, st_src0, st_tgt0, o0, w0))
+    forall ths0 tht0 im_src0 im_tgt0 st_src0 st_tgt0 o0 r_shared0 r_ctx0
+      (INV: I (ths0, tht0, im_src0, im_tgt0, st_src0, st_tgt0, o0, r_shared0))
       tid ths1 tht1
       (THS: TIdSet.add_new tid ths0 ths1)
-      (THT: TIdSet.add_new tid tht0 tht1),
-    exists w1 o1, (<<INV: I (ths1, tht1, im_src0, im_tgt0, st_src0, st_tgt0, o1, w1)>>) /\
-               (<<WORLD: world_le w0 w1>>) /\
-               (forall ths tht im_src1 im_tgt1 st_src st_tgt o w2
-                  (INV: I (ths, tht, im_src1, im_tgt1, st_src, st_tgt, o, w2))
-                  (WORLD: world_le w1 w2),
+      (THT: TIdSet.add_new tid tht0 tht1)
+      (VALID: URA.wf (r_shared0 ⋅ r_ctx0)),
+    exists r_shared1 r_own1 o1, (<<INV: I (ths1, tht1, im_src0, im_tgt0, st_src0, st_tgt0, o1, r_shared1)>>) /\
+               (<<VALID: URA.wf (r_shared1 ⋅ r_own1 ⋅ r_ctx0)>>) /\
+               (forall ths tht im_src1 im_tgt1 st_src st_tgt o r_shared2 r_ctx2
+                  (INV: I (ths, tht, im_src1, im_tgt1, st_src, st_tgt, o, r_shared2))
+                  (VALID: URA.wf (r_shared2 ⋅ r_own1 ⋅ r_ctx2)),
                  forall im_tgt2 (TGT: fair_update im_tgt1 im_tgt2 (sum_fmap_l (tids_fmap tid tht))),
-                 exists im_src2 w3,
+                 exists im_src2,
                    (<<SRC: fair_update im_src1 im_src2 (sum_fmap_l (tids_fmap tid ths))>>) /\
-                     (<<WORLD: world_le w2 w3>>) /\
                      (<<LSIM: forall fs ft,
                          lsim
                            (@local_RR R0 R1 RR tid)
                            tid
                            fs ft
+                           r_own1 r_ctx2
                            src tgt
-                           (ths, tht, im_src2, im_tgt2, st_src, st_tgt, o, w3)
+                           (ths, tht, im_src2, im_tgt2, st_src, st_tgt, o, r_shared2)
                            >>)).
 
   Definition shared_rel_wf (r: shared_rel): Prop :=
-    forall ths tht im_src0 im_tgt0 st_src st_tgt o w0
-      (INV: r (ths, tht, im_src0, im_tgt0, st_src, st_tgt, o, w0)),
+    forall ths tht im_src0 im_tgt0 st_src st_tgt o r_shared0 r_ctx
+           (INV: r (ths, tht, im_src0, im_tgt0, st_src, st_tgt, o, r_shared0))
+           (VALID: URA.wf (r_shared0 ⋅ r_ctx)),
     forall im_tgt1
-      (TGT: fair_update im_tgt0 im_tgt1 (sum_fmap_l (tids_fmap_all ths))),
-    exists im_src1 w1,
+           (TGT: fair_update im_tgt0 im_tgt1 (sum_fmap_l (tids_fmap_all ths))),
+    exists im_src1 r_shared1,
       (<<SRC: fair_update im_src0 im_src1 (sum_fmap_l (tids_fmap_all tht))>>) /\
-        (<<INV: r (ths, tht, im_src1, im_tgt1, st_src, st_tgt, o, w1)>>) /\
-        (<<WORLD: world_le w0 w1>>).
+        (<<INV: r (ths, tht, im_src1, im_tgt1, st_src, st_tgt, o, r_shared1)>>) /\
+        (<<VALID: URA.wf (r_shared1 ⋅ r_ctx)>>).
 
 End PRIMIVIESIM.
 #[export] Hint Constructors __lsim: core.
@@ -482,19 +484,17 @@ Module ModSim.
           wf_tgt_inhabited: inhabited wf_tgt.(T);
           wf_tgt_open: forall (o0: wf_tgt.(T)), exists o1, wf_tgt.(lt) o0 o1;
 
-          world: Type;
-          world_le: world -> world -> Prop;
-          world_le_PreOrder: PreOrder world_le;
+          world: URA.t;
 
-          I: (@shared md_src.(Mod.state) md_tgt.(Mod.state) md_src.(Mod.ident) md_tgt.(Mod.ident) wf_src wf_tgt world) -> Prop;
-          init: forall im_tgt, exists im_src o w,
-            I (NatSet.empty, NatSet.empty, im_src, im_tgt, md_src.(Mod.st_init), md_tgt.(Mod.st_init), o, w);
+          I: (@shared world md_src.(Mod.state) md_tgt.(Mod.state) md_src.(Mod.ident) md_tgt.(Mod.ident) wf_src wf_tgt) -> Prop;
+          init: forall im_tgt, exists im_src o r_shared,
+            I (NatSet.empty, NatSet.empty, im_src, im_tgt, md_src.(Mod.st_init), md_tgt.(Mod.st_init), o, r_shared);
 
           funs: forall fn args, match md_src.(Mod.funs) fn, md_tgt.(Mod.funs) fn with
-                           | None, _ => True
-                           | _, None => False
-                           | Some ktr_src, Some ktr_tgt => local_sim world_le I (@eq Val) (ktr_src args) (ktr_tgt args)
-                           end;
+                                | None, _ => True
+                                | _, None => False
+                                | Some ktr_src, Some ktr_tgt => local_sim I (@eq Val) (ktr_src args) (ktr_tgt args)
+                                end;
         }.
 
   End MODSIM.
